\documentclass[12pt]{article}
\usepackage{mathtools}

\begin{document}

\begin{equation}
 f(x_{i+1}) = f(x_i) + (x_{i+1} - x_i)f^{\prime}(x_i) + \frac{1}{2}(x_{i+1} - x_i)^2 f^{\prime\prime}(x_i) + err(0(h^3))
\end {equation}

\begin{equation}
 f(x_{i-1}) = f(x_i) + (x_{i-1} - x_i) f^{\prime}(x_i) + \frac{1}{2}(x_{i-1} - x_i)^2 f^{\prime\prime}(x_i) + err(0(h^3))
\end {equation}

\noindent For fun(!) subtract equation (2) from (1), recalling that $h = x_{i+1} - x_i$, ...:

\begin{equation}
 f(x_{i+1}) - f(x_{i-1}) = 2hf^{\prime}(x_i) + err(0(h^3))
\end {equation}

\begin{equation}
 f^{\prime}(x_i) = \frac{1}{2h}[f(x_{i+1}) - f(x_{i-1})] + err(0(h^3))
 \end {equation}

\noindent Now try to add (1) and (2) and subtract $2f(x_i)$:

\begin{equation}
 f(x_{i+1}) - 2f(x_i) + f(x_{i-1}) = \frac{1}{2}h^2 f^{\prime\prime}(x_i) + \frac{1}{2}h^2 f^{\prime\prime}(x_i) = h^2 f^{\prime\prime}(x_i) + err(0(h^3))
 \end {equation}
 
 \begin{equation}
  f^{\prime\prime}(x_i) = \frac{f(x_{i+1}) - 2f(x_i) + f(x_{i-1})}{h^2} + err(0(h^3))
 \end {equation}
  
 \noindent Poisson's equation --- Laplace's equation
 
 \begin{equation}
 \frac {\partial^2 f(x)}{\partial x^2} = 4\pi\rho = 0
  \end {equation}
  
 \noindent Solve (6) for $f(x_i)$ (Relaxation/Iterative Method)
 
 \begin{equation}
 f(x_i) = \frac{f(x_{i+1}) + f(x_{i-1})}{2} + err(0(h^3))
  \end {equation}
  
  
\end{document}

